Small refactor

Datalog/Utils.lean
@@ -1,22 +1,14 @@
-def List.product (xs : List α) (len : Nat := 1) : List (List α) :=
+def List.product {α : Type} (xs : List α) (len : Nat) : List (List α) :=
   match len with
   | 0 => [[]]
   | n + 1 => xs.product n |>.flatMap (fun tup => xs.map (fun x => x :: tup))
 
 #eval [1, 2, 3].product 0
-#eval [1, 2, 3].product
+#eval [1, 2, 3].product 1
 #eval [1, 2, 3].product 3
 
-theorem List.mem_product_iff (xs : List α) (len : Nat) :
-    ∀ tup, tup ∈ xs.product len ↔ tup.length = len ∧ ∀ e ∈ tup, e ∈ xs := by
-  intro tup
+theorem List.mem_product_iff {α : Type} (xs : List α) (len : Nat) (tup : List α) :
+    tup ∈ xs.product len ↔ tup.length = len ∧ ∀ e ∈ tup, e ∈ xs := by
   induction len generalizing tup with
-  | zero =>
-    simp [List.product]
-    grind
-  | succ n ih =>
-    constructor <;> intro h
-    · simp [List.product] at h
-      grind
-    · simp [List.product]
-      cases tup with grind
+  | zero => grind [List.product]
+  | succ n ih => cases tup with grind [List.product]
