Datalog/Spec.lean
@@ -1,0 +1,134 @@
+import Datalog.Syntax
+import Datalog.DSL
+import Datalog.Utils
+
+-- Substitution
+
+abbrev Substitution :=
+  String → String
+
+def Term.applySub (σ : Substitution) : Term → Term
+  | .const c => .const c
+  | .var v => .const (σ v)
+
+def Atom.applySub (σ : Substitution) (atom : Atom) : Atom :=
+  Atom.mk atom.rel (atom.terms.map (Term.applySub σ))
+
+theorem isConst_of_mem_applySub {term : Term} {atom : Atom} {σ : Substitution} (h : term ∈ (atom.applySub σ).terms) :
+    term.isConst := by
+  simp [Atom.applySub, Term.applySub] at h
+  simp [Term.isConst]
+  grind
+
+-- Predicates
+
+def Program.Predicates (prog : Program) (pred : String × Nat) : Prop :=
+  ∃ r ∈ prog, pred = r.head.predicate ∨ ∃ a ∈ r.body, pred = a.predicate
+
+theorem Program.mem_getPredicates_iff (prog : Program) (pred : String × Nat) :
+    pred ∈ prog.getPredicates ↔ prog.Predicates pred := by
+  simp [Program.getPredicates, Rule.getPredicates, Atom.predicate, Program.Predicates]
+  grind
+
+-- Constants
+
+def Program.Constants (prog : Program) (t : Term) : Prop :=
+  t.isConst ∧ ∃ r ∈ prog, t ∈ r.head.terms ∨ ∃ a ∈ r.body, t ∈ a.terms
+
+theorem Program.mem_getConstants_iff (prog : Program) (term : Term) :
+    term ∈ prog.getConstants ↔ prog.Constants term := by
+  simp [Program.getConstants, Rule.getConstants, Atom.getConstants, Program.Constants]
+  grind
+
+-- Herbrand base
+
+def Program.HerbrandBase (prog : Program) (a : Atom) : Prop :=
+  prog.Predicates a.predicate ∧ ∀ t ∈ a.terms, prog.Constants t
+
+theorem Program.mem_getHerbrandBase_iff (prog : Program) (atom : Atom) :
+    atom ∈ prog.getHerbrandBase ↔ prog.HerbrandBase atom := by
+  simp [Program.getHerbrandBase, Program.mem_getPredicates_iff, List.mem_product_iff, Program.mem_getConstants_iff, Program.HerbrandBase, Atom.predicate]
+  grind
+
+-- Herbrand model
+
+inductive Program.HerbrandModel (prog : Program) : Atom → Prop where
+  | step : {r : Rule} → r ∈ prog → (σ : Substitution) → ({a : Atom} → a ∈ r.body → prog.HerbrandModel (a.applySub σ)) → prog.HerbrandModel (r.head.applySub σ)
+
+-- Safety
+
+def Rule.IsSafe (rule : Rule) : Prop :=
+  ∀ t ∈ rule.head.terms, t.isVar → ∃ a ∈ rule.body, t ∈ a.terms
+
+def Program.IsSafe (prog : Program) : Prop :=
+  ∀ r ∈ prog, r.IsSafe
+
+example : Program.IsSafe [Prog|
+parent(xerces, brooke).
+parent(brooke, damocles).
+ancestor(X, Y) :- parent(X, Y).
+ancestor(X, Y) :- parent(X, Z), ancestor(Z, Y).
+] := by simp [Program.IsSafe, Rule.IsSafe, Term.isVar]
+
+-- Finiteness
+
+theorem HerbrandModel_subseteq_HerbrandBase (prog : Program) (safety : prog.IsSafe) (atom : Atom) :
+    prog.HerbrandModel atom → prog.HerbrandBase atom := by
+  intro h
+  induction h with
+  | step hr σ hbody ih =>
+    rename_i r
+    constructor
+    · simp [Program.Predicates, Atom.predicate, Atom.applySub]
+      grind
+    · intro t ht
+      constructor
+      · exact isConst_of_mem_applySub ht
+      · cases Classical.em (t ∈ r.head.terms) with
+        | inl hhead => exact ⟨r, hr, .inl hhead⟩
+        | inr hhead =>
+          have ⟨s, hs⟩ : ∃ s, .var s ∈ r.head.terms ∧ .const (σ s) = t := by
+            simp [Atom.applySub, Term.applySub, List.mem_map] at ht
+            grind
+          have ⟨a, ha⟩ := (safety r hr) (.var s) hs.left (by simp [Term.isVar])
+          have : t ∈ (a.applySub σ).terms := by
+            simp [Atom.applySub, Term.applySub]
+            grind
+          simp [Program.HerbrandBase, Program.Constants] at ih
+          grind
+
+-- Fixpoint semantics
+
+def Subseteq {α : Type} (s₁ s₂ : α → Prop) : Prop :=
+  ∀ e, s₁ e → s₂ e
+
+infix:50 " ⊆ " => Subseteq
+
+def Program.ImmediateConsequence (prog : Program) (db : Atom → Prop) (atom : Atom) : Prop :=
+  ∃ r ∈ prog, ∃ σ, r.head.applySub σ = atom ∧ ∀ a ∈ r.body, db (a.applySub σ)
+
+def Program.LeastFixedPoint (prog : Program) (atom : Atom) : Prop :=
+  ∀ db, prog.ImmediateConsequence db ⊆ db → db atom
+
+theorem ImmediateConsequence_monotonic (prog : Program) :
+    ∀ db₁ db₂, db₁ ⊆ db₂ → prog.ImmediateConsequence db₁ ⊆ prog.ImmediateConsequence db₂ := by
+  intro db₁ db₂ h
+  simp [Subseteq, Program.ImmediateConsequence]
+  intro a r hr σ hσ hbody
+  refine ⟨r, hr, σ, hσ, ?_⟩
+  simp [Subseteq] at h
+  grind
+
+theorem HerbrandModel_iff_LeastFixedPoint (prog : Program) (atom : Atom) :
+    prog.HerbrandModel atom ↔ prog.LeastFixedPoint atom := by
+  constructor
+  · intro h db hdb
+    induction h with
+    | step hr σ _ ih =>
+      apply hdb
+      exact ⟨_, hr, σ, rfl, fun _ => ih⟩
+  · intro h
+    apply h
+    intro a ⟨r, hr, σ, hσ, hbody⟩
+    rw [← hσ]
+    apply Program.HerbrandModel.step hr _ (fun {a} ha => hbody a ha)
