Datalog/Syntax.lean
@@ -1,0 +1,87 @@
+import Datalog.Utils
+
+-- Term
+
+inductive Term where
+  | const : String → Term
+  | var : String → Term
+  deriving BEq
+
+instance : ToString Term where
+  toString
+    | .const c => c
+    | .var v => v
+
+def Term.isConst : Term → Bool
+  | .const _ => true
+  | _ => false
+
+def Term.isVar : Term → Bool
+  | .var _ => true
+  | _ => false
+
+def Term.isGround : Term → Bool :=
+  Term.isConst
+
+-- Atom
+
+structure Atom where
+  rel : String
+  terms : List Term
+  deriving BEq
+
+instance : ToString Atom where
+  toString
+    | Atom.mk rel [] => rel
+    | Atom.mk rel terms => rel ++ "(" ++ ", ".intercalate (terms.map toString) ++ ")"
+
+def Atom.predicate (atom : Atom) : String × Nat :=
+  (atom.rel, atom.terms.length)
+
+def Atom.getConstants (atom : Atom) : List Term :=
+  atom.terms.filter Term.isConst
+
+def Atom.isGround (atom : Atom) : Bool :=
+  ∀ t ∈ atom.terms, t.isGround
+
+-- Rule
+
+structure Rule where
+  head : Atom
+  body : List Atom
+  deriving BEq
+
+instance : ToString Rule where
+  toString
+    | Rule.mk head [] => toString head ++ "."
+    | Rule.mk head body => toString head ++ " :- " ++ ", ".intercalate (body.map toString) ++ "."
+
+def Rule.getPredicates (rule : Rule) : List (String × Nat) :=
+  rule.head.predicate :: rule.body.map Atom.predicate
+
+def Rule.getConstants (rule : Rule) : List Term :=
+  rule.head.getConstants ++ rule.body.flatMap Atom.getConstants
+
+def Rule.isGround (rule : Rule) : Bool :=
+  rule.head.isGround ∧ ∀ a ∈ rule.body, a.isGround
+
+def Rule.isFact (rule : Rule) : Bool :=
+  rule.body.isEmpty
+
+-- Program
+
+abbrev Program :=
+  List Rule
+
+instance : ToString Program where
+  toString prog :=
+    "\n".intercalate (prog.map toString)
+
+def Program.getPredicates (prog : Program) : List (String × Nat) :=
+  prog.flatMap Rule.getPredicates
+
+def Program.getConstants (prog : Program) : List Term :=
+  prog.flatMap Rule.getConstants
+
+def Program.getHerbrandBase (prog : Program) : List Atom :=
+  prog.getPredicates.flatMap (fun (rel, arity) => prog.getConstants.product arity |>.map (fun terms => Atom.mk rel terms))
